found a bug in proof

src/drf/DRF_PF3.v
@@ -42,11 +42,6 @@ Set Implicit Arguments.
 
 
 
-(* Inductive my_caps (mem0 prom : Memory.t) (l : Loc.t) (t from : Time.t) (msg : Message.t) := *)
-(*   (<<CAPS: caps mem0 prom l t from msg>>) /\ *)
-(*   (<< *)
-
-
 Definition wf_time_evt (P: Loc.t -> Time.t -> Prop) (e: ThreadEvent.t) : Prop :=
   match e with
   | ThreadEvent.promise loc from to msg kind =>
@@ -112,722 +107,6 @@ Proof.
       eapply wf_time_evt_mon; eauto.
       i. ss. eapply List.in_or_app; eauto.
 Qed.
-
-(* Definition self_latest_reseves_loc (mem prom: Memory.t) (loc: Loc.t): Prop := *)
-(*   Memory.latest_reserve loc mem prom. *)
-
-Definition other_latest_reserves (L: Loc.t -> Prop)
-           (mem: Memory.t) (loc: Loc.t) (to: Time.t) (from: Time.t) :=
-  (<<LATEST: to = Memory.max_ts loc mem>>) /\
-  (<<RESERVE: Memory.get loc to mem = Some (from, Message.reserve)>>) /\
-  (<<OTHER: L loc>>)
-.
-
-Definition other_latest_reserves_times (L: Loc.t -> Prop)
-           (mem: Memory.t) (loc: Loc.t) (to: Time.t): Prop :=
-  exists from,
-    (<<RESERVE: other_latest_reserves L mem loc to from>>).
-
-Definition other_caps (L: Loc.t -> Prop)
-           (mem0 mem1: Memory.t) (loc: Loc.t) (to: Time.t) (from: Time.t) :=
-  (<<FULL: Memory.max_full_ts mem0 loc from>>) /\
-  (<<LATEST: exists from0 val released,
-      (<<CAP: caps mem0 mem1 loc to from0 (Message.full val released)>>)>>) /\
-  (<<OTHER: L loc>>)
-.
-
-Definition other_caps_times (L: Loc.t -> Prop)
-           (mem0 mem1: Memory.t) (loc: Loc.t) (to: Time.t) :=
-  exists from,
-    (<<CAP: other_caps L mem0 mem1 loc to from>>).
-
-Definition times_in_memory (mem: Memory.t) (L: Loc.t -> list Time.t): Prop :=
-  forall loc t,
-    (<<SAT: List.In t (L loc)>>) <->
-    (<<INMEMORY:
-       (exists from msg, (<<GET: Memory.get loc t mem = Some (from, msg)>>)) \/
-       (exists to msg, (<<GET: Memory.get loc to mem = Some (t, msg)>>))>>).
-
-Lemma times_in_memory_exists mem
-  :
-    exists l, times_in_memory mem l.
-Proof.
-  hexploit (choice
-              (fun loc tl =>
-                 forall t,
-                   (<<SAT: List.In t tl>>) <->
-                   (<<INMEMORY:
-                      (exists from msg, (<<GET: Memory.get loc t mem = Some (from, msg)>>)) \/
-                      (exists to msg, (<<GET: Memory.get loc to mem = Some (t, msg)>>))>>))); auto.
-  intros loc.
-  hexploit (wf_cell_msgs_exists (mem loc)). i. des.
-  exists ((List.map (fun ftm =>
-                       match ftm with
-                       | (from, _, _) => from
-                       end) l)
-            ++
-            (List.map (fun ftm =>
-                         match ftm with
-                         | (_, to, _) => to
-                         end) l)).
-  i. split; i.
-  - red in H. eapply List.in_app_or in H. des.
-    + eapply List.in_map_iff in H. des.
-      destruct x as [[from to] msg]. clarify.
-      eapply COMPLETE in H0. right. eauto.
-    + eapply List.in_map_iff in H. des.
-      destruct x as [[from to] msg]. clarify.
-      eapply COMPLETE in H0. left. eauto.
-  - eapply List.in_or_app.  des.
-    + right. eapply COMPLETE in GET.
-      eapply List.in_map_iff. esplits; eauto. ss.
-    + left. eapply COMPLETE in GET.
-      eapply List.in_map_iff. esplits; eauto. ss.
-Qed.
-
-Inductive caps_collapsing (L: Loc.t -> Prop)
-          (mem: Memory.t): Loc.t -> Time.t -> Time.t -> Prop :=
-| caps_collapsing_not_in
-    loc t
-    (NSAT: ~ L loc)
-  :
-    caps_collapsing L mem loc t t
-| caps_collapsing_in_memory
-    loc t max
-    (SAT: L loc)
-    (FULL: Memory.max_full_ts mem loc max)
-    (TLE: Time.le t max)
-  :
-    caps_collapsing L mem loc t t
-| caps_collapsing_latest_reserve
-    loc t max
-    (SAT: L loc)
-    (FULL: Memory.max_full_ts mem loc max)
-    (MAX: t = Memory.max_ts loc mem)
-  :
-    caps_collapsing L mem loc max t
-| caps_collapsing_cap
-    loc t max
-    (SAT: L loc)
-    (FULL: Memory.max_full_ts mem loc max)
-    (CAP: t = Time.incr (Memory.max_ts loc mem))
-  :
-    caps_collapsing L mem loc max t
-| caps_collapsing_outer_memory
-    loc t
-    (SAT: L loc)
-    (TLE: Time.lt (Time.incr (Memory.max_ts loc mem)) t)
-  :
-    caps_collapsing L mem loc t t
-.
-
-Lemma forget_memory_get P mem0 mem1 loc to msg
-      (FORGET: forget_memory P mem0 mem1)
-      (GET: Memory.get loc to mem0 = Some msg)
-  :
-    (<<NOT: ~ P loc to>>) /\ (<<GET: Memory.get loc to mem1 = Some msg>>).
-Proof.
-  inv FORGET. destruct (classic (P loc to)).
-  - exfalso. rewrite FORGET0 in GET; auto. clarify.
-  - esplits; eauto.
-    rewrite <- COMPLETE; auto.
-Qed.
-
-Lemma caps_get_reserve mem0 prom mem1 loc to from
-      (RESERVE: Memory.reserve_wf prom mem0)
-      (INHABITED: Memory.inhabited mem0)
-      (CLOSED: Memory.closed mem0)
-      (CAP: Memory.cap prom mem0 mem1)
-      (CAPS: caps mem0 mem1 loc to from Message.reserve)
-  :
-    exists from0 to1 msg0 msg1,
-      (<<GET0: Memory.get loc from mem0 = Some (from0, msg0)>>) /\
-      (<<GET1: Memory.get loc to1 mem0 = Some (to, msg1)>>) /\
-      (<<SPACE: forall t (ITV: Interval.mem (from, to) t), ~ covered loc t mem0>>)
-.
-Proof.
-  unfold caps in CAPS. des. inv CAP.
-  exploit COMPLETE; eauto. i. des.
-  set (@cell_elements_least
-         (mem0 loc)
-         (fun t => Time.lt from t)). des.
-  - hexploit (MIDDLE loc f from from0 to0).
-    { econs; eauto. i.
-      destruct (Memory.get loc ts mem0) eqn:GET2; auto. destruct p.
-      exfalso. exploit LEAST.
-      - eapply GET2.
-      - eauto.
-      - i. exploit Memory.get_ts; try apply GET.
-        i. des; clarify.
-        + eapply Time.lt_strorder. eapply TimeFacts.lt_le_lt.
-          * eapply SAT.
-          * eapply Time.bot_spec.
-        + eapply Time.lt_strorder. eapply TimeFacts.le_lt_lt.
-          * etrans.
-            { eapply x1. }
-            { eapply TS2. }
-          * eauto. }
-    { exploit memory_get_from_mon.
-      - eapply x.
-      - eapply GET.
-      - eauto.
-      - i. destruct x2; auto. destruct H. exfalso.
-        exploit memory_get_from_inj.
-        { eapply SOUND. eapply GET. }
-        { eapply GET1. }
-        i. des; clarify.
-        + setoid_rewrite GET0 in GET. clarify.
-        + eapply Time.lt_strorder; eauto. }
-    i. exploit memory_get_from_inj.
-    { eapply H. }
-    { eapply GET1. }
-    i. des; clarify.
-    + esplits; eauto. ii. inv H0.
-      exploit Memory.get_disjoint.
-      * eapply SOUND. eapply GET2.
-      * eapply H.
-      * i. des; clarify. eapply x2; eauto.
-    + specialize (INHABITED loc).
-      eapply SOUND in INHABITED. clarify.
-  - exploit Memory.max_ts_spec.
-    { eapply x. }
-    i. des. destruct MAX.
-    + exfalso. eapply EMPTY; eauto.
-    + unfold Time.eq in *. subst. exploit x0; auto. intros LATEST.
-      exploit Memory.latest_val_exists; eauto. i. des.
-      exploit Memory.max_full_view_exists; eauto. i. des.
-      exploit BACK; eauto. i.
-      exploit memory_get_from_inj.
-      * eapply x1.
-      * eapply GET1.
-      * i. des; clarify.
-        { exfalso. eapply Time.lt_strorder. eapply TimeFacts.lt_le_lt.
-          - eapply Time.incr_spec.
-          - rewrite BOT0. eapply Time.bot_spec. }
-        { erewrite INHABITED in GET0. clarify. }
-Qed.
-
-Definition memory_concrete_le (lhs rhs: Memory.t): Prop :=
-  forall loc to from val released
-         (GET: Memory.get loc to lhs = Some (from, Message.full val released)),
-    Memory.get loc to rhs = Some (from, Message.full val released).
-
-Lemma memory_concrete_le_le
-  :
-    Memory.le <2= memory_concrete_le.
-Proof.
-  ii. eauto.
-Qed.
-Hint Resolve memory_concrete_le_le.
-
-Lemma memory_concrete_le_closed_timemap tm mem0 mem1
-      (MLE: memory_concrete_le mem0 mem1)
-      (TM: Memory.closed_timemap tm mem0)
-  :
-    Memory.closed_timemap tm mem1.
-Proof.
-  ii. hexploit (TM loc). i. des.
-  esplits; eauto.
-Qed.
-
-Lemma memory_concrete_le_closed_view vw mem0 mem1
-      (MLE: memory_concrete_le mem0 mem1)
-      (VW: Memory.closed_view vw mem0)
-  :
-    Memory.closed_view vw mem1.
-Proof.
-  inv VW. econs.
-  - eapply memory_concrete_le_closed_timemap; eauto.
-  - eapply memory_concrete_le_closed_timemap; eauto.
-Qed.
-
-Lemma memory_concrete_le_closed_opt_view vw mem0 mem1
-      (MLE: memory_concrete_le mem0 mem1)
-      (VW: Memory.closed_opt_view vw mem0)
-  :
-    Memory.closed_opt_view vw mem1.
-Proof.
-  inv VW; econs.
-  eapply memory_concrete_le_closed_view; eauto.
-Qed.
-
-Lemma memory_concrete_le_closed_msg msg mem0 mem1
-      (MLE: memory_concrete_le mem0 mem1)
-      (MSG: Memory.closed_message msg mem0)
-  :
-    Memory.closed_message msg mem1.
-Proof.
-  inv MSG; econs.
-  eapply memory_concrete_le_closed_opt_view; eauto.
-Qed.
-
-Lemma memory_concrete_le_closed_tview vw mem0 mem1
-      (MLE: memory_concrete_le mem0 mem1)
-      (VW: TView.closed vw mem0)
-  :
-    TView.closed vw mem1.
-Proof.
-  inv VW. econs.
-  - i. eapply memory_concrete_le_closed_view; eauto.
-  - eapply memory_concrete_le_closed_view; eauto.
-  - eapply memory_concrete_le_closed_view; eauto.
-Qed.
-
-Lemma memory_concrete_le_reserve_wf prom mem0 mem1
-      (MLE: memory_concrete_le mem0 mem1)
-      (RESERVE: Memory.reserve_wf prom mem0)
-  :
-    Memory.reserve_wf prom mem1.
-Proof.
-  ii. eapply RESERVE in GET. des.
-  esplits; eauto.
-Qed.
-
-Lemma memory_concrete_le_local_wf lc mem0 mem1
-      (MLE: memory_concrete_le mem0 mem1)
-      (PROM: Memory.le (Local.promises lc) mem1)
-      (LOCAL: Local.wf lc mem0)
-  :
-    Local.wf lc mem1.
-Proof.
-  inv LOCAL. econs; eauto.
-  - eapply memory_concrete_le_closed_tview; eauto.
-  - eapply memory_concrete_le_reserve_wf; eauto.
-Qed.
-
-Lemma partial_cap_closed prom mem0 mem1 mem2
-      (MLE: Memory.le prom mem0)
-      (CLOSED: Memory.closed mem0)
-      (RESERVEWF: Memory.reserve_wf prom mem0)
-      (INHABITED: Memory.inhabited mem0)
-      (CAP: Memory.cap prom mem0 mem2)
-      (MLE0: Memory.le mem0 mem1)
-      (MLE1: Memory.le mem1 mem2)
-  :
-    Memory.closed mem1.
-Proof.
-  exploit Memory.max_full_timemap_exists; eauto. intros [tm MAX].
-  inv CLOSED. econs; eauto.
-  i. destruct (Memory.get loc to mem0) as [[from0 msg0]|] eqn:GET.
-  - dup GET. eapply MLE0 in GET. clarify.
-    eapply CLOSED0 in GET0. des. esplits; eauto.
-    eapply memory_concrete_le_closed_msg; eauto.
-  - destruct msg.
-    + eapply MLE1 in MSG.
-      exploit caps_max_view; eauto.
-      * econs; eauto.
-      * i. des; clarify. esplits; eauto.
-        { econs; eauto. econs; eauto. econs. refl. }
-        { econs; eauto. ss. transitivity (Memory.max_ts loc mem0).
-          - specialize (MAX loc). inv MAX. des.
-            eapply Memory.max_ts_spec in GET0. des. eauto.
-          - left. eapply Time.incr_spec. }
-        { eapply memory_concrete_le_closed_msg; eauto.
-          econs. econs. econs.
-          - eapply Memory.max_full_timemap_closed; eauto.
-          - eapply Memory.max_full_timemap_closed; eauto. }
-    + esplits; eauto. econs.
-Qed.
-
-Lemma other_caps_forget_le
-      mem0 mem1 mem2 prom (L: Loc.t -> Prop)
-      (CAP: Memory.cap prom mem0 mem2)
-      (FORGET: forget_memory (other_latest_reserves_times L mem0 \2/ other_caps_times L mem0 mem1) mem1 mem2)
-  :
-    memory_concrete_le mem0 mem1.
-Proof.
-  inv FORGET. ii.
-  erewrite COMPLETE.
-  - eapply Memory.cap_le in CAP; eauto. refl.
-  - ii. des.
-    + unfold other_latest_reserves_times in *. des.
-      inv RESERVE. des. clarify.
-    + unfold other_caps_times in *. des.
-      inv CAP0. des. unfold caps in CAP0. des. clarify.
-Qed.
-
-Lemma other_caps_forget_prom_le
-      mem0 mem1 mem2 prom (L: Loc.t -> Prop)
-      (OTHERS: forall loc (SAT: L loc), Memory.latest_reserve loc prom mem0)
-      (MLE: Memory.le prom mem0)
-      (CLOSED: Memory.closed mem0)
-      (RESERVEWF: Memory.reserve_wf prom mem0)
-      (INHABITED: Memory.inhabited mem0)
-      (CAP: Memory.cap prom mem0 mem2)
-      (FORGET: forget_memory (other_latest_reserves_times L mem0 \2/ other_caps_times L mem0 mem1) mem1 mem2)
-  :
-    Memory.le prom mem1.
-Proof.
-  inv FORGET. ii.
-  erewrite COMPLETE.
-  - eapply Memory.cap_le in CAP; eauto.
-  - ii. des.
-    + unfold other_latest_reserves_times in *. des.
-      inv RESERVE. des. clarify.
-      dup LHS. eapply MLE in LHS0. clarify.
-      eapply OTHERS in OTHER. unfold Memory.latest_reserve in OTHER.
-      rewrite LHS in *. clarify.
-    + unfold other_caps_times in *. des.
-      inv CAP0. des. unfold caps in CAP0. des.
-      eapply MLE in LHS; eauto. clarify.
-Qed.
-
-Lemma identity_mapped_view tm maxmap (f: Loc.t -> Time.t -> Time.t -> Prop)
-      (TM: TimeMap.le tm maxmap)
-      (IDENT: forall loc ts (TS: Time.le ts (maxmap loc)), f loc ts ts)
-  :
-    timemap_map f tm tm.
-Proof.
-  ii. eapply IDENT; eauto.
-Qed.
-
-Lemma caps_collapsing_ident L mem loc maxts ts
-      (MAX: Memory.max_full_ts mem loc maxts)
-      (TS: Time.le ts maxts)
-  :
-    (caps_collapsing L mem) loc ts ts.
-Proof.
-  i. destruct (classic (L loc)).
-  - econs 2; eauto.
-  - econs 1; eauto.
-Qed.
-
-Definition memory_reserve_wf mem := Memory.reserve_wf mem mem.
-
-Lemma memory_reserve_wf_promise
-      prom0 mem0 loc from to msg prom1 mem1 kind
-      (PROMISE: Memory.promise prom0 mem0 loc from to msg prom1 mem1 kind)
-      (RESERVE: memory_reserve_wf mem0)
-  :
-    memory_reserve_wf mem1.
-Proof.
-  inv PROMISE.
-  - ii. erewrite Memory.add_o in GET; eauto. des_ifs.
-    + ss; des; clarify. exploit RESERVE0; eauto.
-      i. des. eapply Memory.add_get1 in x; eauto.
-    + eapply RESERVE in GET; eauto. clear o. des.
-      eapply Memory.add_get1 in GET; eauto.
-  - ii. des. clarify. erewrite Memory.split_o in GET; eauto. des_ifs.
-    + ss; des; clarify. eapply Memory.split_get0 in MEM. des.
-      esplits; eauto.
-    + eapply RESERVE in GET; eauto. clear o o0. des.
-      eapply Memory.split_get1 in GET; eauto. des. esplits; eauto.
-  - ii. erewrite Memory.lower_o in GET; eauto. des_ifs.
-    + ss; des; clarify. inv MEM. inv LOWER. inv MSG_LE.
-    + eapply RESERVE in GET; eauto. clear o. des.
-      eapply Memory.lower_get1 in GET; eauto. des.
-      inv MSG_LE. esplits; eauto.
-  - ii. erewrite Memory.remove_o in GET; eauto. des_ifs. guardH o.
-    dup MEM. eapply Memory.remove_get0 in MEM0. des.
-    eapply RESERVE in GET; eauto. des. dup GET.
-    eapply Memory.remove_get1 in GET2; eauto. ss. des; clarify.
-    esplits; eauto.
-Qed.
-
-Lemma memory_reserve_wf_tstep lang (th0 th1: Thread.t lang) tf e
-      (RESERVE: memory_reserve_wf th0.(Thread.memory))
-      (STEP: Thread.step tf e th0 th1)
-  :
-    memory_reserve_wf th1.(Thread.memory).
-Proof.
-  inv STEP; inv STEP0; ss.
-  - inv LOCAL. eapply memory_reserve_wf_promise; eauto.
-  - inv LOCAL; eauto.
-    + inv LOCAL0. inv WRITE.
-      eapply memory_reserve_wf_promise; eauto.
-    + inv LOCAL1. inv LOCAL2. inv WRITE.
-      eapply memory_reserve_wf_promise; eauto.
-Qed.
-
-Lemma memory_reserve_wf_tsteps lang (th0 th1: Thread.t lang)
-      (RESERVE: memory_reserve_wf th0.(Thread.memory))
-      (STEP: rtc (tau (@Thread.step_allpf lang)) th0 th1)
-  :
-    memory_reserve_wf th1.(Thread.memory).
-Proof.
-  ginduction STEP; eauto.
-  i. eapply IHSTEP; eauto. inv H. inv TSTEP.
-  eapply memory_reserve_wf_tstep; eauto.
-Qed.
-
-Lemma memory_reserve_wf_init
-  :
-    memory_reserve_wf Memory.init.
-Proof.
-  ii. unfold Memory.get, Memory.init in *. ss.
-  rewrite Cell.init_get in GET. des_ifs.
-Qed.
-
-Lemma memory_reserve_wf_configuration_step c0 c1 e tid
-      (RESERVE: memory_reserve_wf c0.(Configuration.memory))
-      (STEP: Configuration.step e tid c0 c1)
-  :
-    memory_reserve_wf c1.(Configuration.memory).
-Proof.
-  eapply configuration_step_equivalent in STEP. inv STEP. ss.
-  eapply memory_reserve_wf_tstep in STEP0; eauto.
-  eapply memory_reserve_wf_tsteps in STEPS; eauto.
-Qed.
-
-Lemma not_latest_reserve_le_max_full_ts loc mem ts to from msg
-      (RESERVEWF : memory_reserve_wf mem)
-      (INHABITED : Memory.inhabited mem)
-      (MAX : Memory.max_full_ts mem loc ts)
-      (GET: Memory.get loc to mem = Some (from, msg))
-  :
-    (<<TLE: Time.le to ts>>) \/
-    ((<<TO: to = Memory.max_ts loc mem>>) /\
-     (<<FROM: from = ts>>) /\
-     (<<MSG: msg = Message.reserve>>)).
-Proof.
-  inv MAX. des.
-  destruct msg.
-  - left. eapply MAX0; eauto.
-  - exploit RESERVEWF; eauto. i. des.
-    destruct (TimeFacts.le_lt_dec to ts); auto.
-    dup x. eapply MAX0 in x; eauto. destruct x.
-    + exfalso. exploit memory_get_from_mon.
-      { eapply GET0. }
-      { eapply GET. }
-      { auto. }
-      i. eapply Time.lt_strorder. eapply TimeFacts.le_lt_lt.
-      * eapply x1.
-      * eapply H.
-    + unfold Time.eq in *. subst. right. esplits; eauto.
-      setoid_rewrite GET0 in x0. clarify.
-      dup GET. eapply Memory.max_ts_spec in GET1. des.
-      destruct MAX; auto. exfalso.
-      destruct msg.
-      * eapply MAX0 in GET2. eapply Time.lt_strorder.
-        eapply TimeFacts.lt_le_lt.
-        { etrans.
-          - eapply l.
-          - eapply H. }
-        { eauto. }
-      * dup GET2. eapply RESERVEWF in GET2. des.
-        eapply MAX0 in GET2.
-        exploit memory_get_from_mon.
-        { eapply GET. }
-        { eapply GET1. }
-        { eapply H. }
-        i. eapply Time.lt_strorder.
-        eapply TimeFacts.lt_le_lt.
-        { eapply l. }
-        { etrans.
-          - eapply x0.
-          - eapply Memory.get_ts in GET1. des; clarify. }
-Qed.
-
-Lemma max_full_ts_le_max_ts mem loc ts
-      (MAX: Memory.max_full_ts mem loc ts)
-  :
-    Time.le ts (Memory.max_ts loc mem).
-Proof.
-  inv MAX. des.
-  eapply Memory.max_ts_spec in GET. des; auto.
-Qed.
-
-Lemma max_full_ts_max_ts loc mem ts
-      (RESERVEWF : memory_reserve_wf mem)
-      (INHABITED : Memory.inhabited mem)
-      (MAX : Memory.max_full_ts mem loc ts)
-  :
-    (<<FULL: ts = Memory.max_ts loc mem>>) \/
-    ((<<TLT: Time.lt ts (Memory.max_ts loc mem)>>) /\
-     (<<GET: Memory.get loc (Memory.max_ts loc mem) mem = Some (ts, Message.reserve)>>)).
-Proof.
-  dup MAX. inv MAX. des.
-  eapply Memory.max_ts_spec in GET. des.
-  dup GET0. eapply not_latest_reserve_le_max_full_ts in GET0; eauto.
-  des; clarify.
-  - left. eapply TimeFacts.antisym; eauto.
-  - right. split; eauto. dup GET1.
-    eapply memory_get_ts_strong in GET1. des; clarify.
-    erewrite GET2 in *.
-    erewrite INHABITED in GET0. clarify.
-Qed.
-
-Lemma caps_collapsing_ident2 L mem maxts loc ts fts
-      (MAX: Memory.max_full_ts mem loc maxts)
-      (TS: Time.le fts maxts)
-      (MAP: (caps_collapsing L mem) loc ts fts)
-  :
-    ts = fts.
-Proof.
-  inv MAP; eauto.
-  - exploit Memory.max_full_ts_inj.
-    { eapply FULL. }
-    { eapply MAX. }
-    i. clarify. eapply TimeFacts.antisym; auto.
-    eapply max_full_ts_le_max_ts in FULL; auto.
-  - exfalso. eapply max_full_ts_le_max_ts in FULL. exfalso.
-    eapply Time.lt_strorder. eapply TimeFacts.lt_le_lt.
-    + eapply DenseOrder.DenseOrder.incr_spec.
-    + etrans.
-      * eapply TS.
-      * eapply max_full_ts_le_max_ts; eauto.
-Qed.
-
-Lemma caps_collapsing_ident3 L mem maxts loc ts fts
-      (RESERVEWF : memory_reserve_wf mem)
-      (INHABITED : Memory.inhabited mem)
-      (MAX: Memory.max_full_ts mem loc maxts)
-      (TS: Time.lt ts maxts)
-      (MAP: (caps_collapsing L mem) loc ts fts)
-  :
-    ts = fts.
-Proof.
-  inv MAP; eauto.
-  - exploit Memory.max_full_ts_inj.
-    { eapply FULL. }
-    { eapply MAX. }
-    i. clarify. exfalso. eapply Time.lt_strorder; eauto.
-  - exploit Memory.max_full_ts_inj.
-    { eapply FULL. }
-    { eapply MAX. }
-    i. clarify. exfalso. eapply Time.lt_strorder; eauto.
-Qed.
-
-Lemma caps_collapsing_timemap L mem tm
-      (INHABITED: Memory.inhabited mem)
-      (TM: Memory.closed_timemap tm mem)
-  :
-    timemap_map (caps_collapsing L mem) tm tm.
-Proof.
-  exploit Memory.max_full_timemap_exists; eauto. intros [maxmap MAX].
-  eapply identity_mapped_view.
-  - eapply Memory.max_full_timemap_spec; eauto.
-  - i. eapply caps_collapsing_ident; eauto.
-Qed.
-
-Lemma caps_collapsing_view L mem vw
-      (INHABITED: Memory.inhabited mem)
-      (VW: Memory.closed_view vw mem)
-  :
-    view_map (caps_collapsing L mem) vw vw.
-Proof.
-  inv VW. econs.
-  - eapply caps_collapsing_timemap; eauto.
-  - eapply caps_collapsing_timemap; eauto.
-Qed.
-
-Lemma caps_collapsing_opt_view L mem vw
-      (INHABITED: Memory.inhabited mem)
-      (VW: Memory.closed_opt_view vw mem)
-  :
-    opt_view_map (caps_collapsing L mem) vw vw.
-Proof.
-  inv VW; econs.
-  eapply caps_collapsing_view; eauto.
-Qed.
-
-Lemma caps_collapsing_message L mem msg
-      (INHABITED: Memory.inhabited mem)
-      (MSG: Memory.closed_message msg mem)
-  :
-    msg_map (caps_collapsing L mem) msg msg.
-Proof.
-  inv MSG; econs.
-  eapply caps_collapsing_opt_view; eauto.
-Qed.
-
-Lemma caps_collapsing_tview L mem vw
-      (INHABITED: Memory.inhabited mem)
-      (VW: TView.closed vw mem)
-  :
-    tview_map (caps_collapsing L mem) vw vw.
-Proof.
-  inv VW. econs.
-  - i. eapply caps_collapsing_view; eauto.
-  - eapply caps_collapsing_view; eauto.
-  - eapply caps_collapsing_view; eauto.
-Qed.
-
-Lemma caps_collapsing_promises (L: Loc.t -> Prop) mem prom
-      (MLE: Memory.le prom mem)
-      (CLOSED: Memory.closed mem)
-      (RESERVEWF: memory_reserve_wf mem)
-      (INHABITED: Memory.inhabited mem)
-      (LATESTRESERVE: forall
-          loc (SAT: L loc)
-          from msg
-          (GET: Memory.get loc (Memory.max_ts loc mem) prom = Some (from, msg)),
-          msg <> Message.reserve)
-  :
-    promises_map (caps_collapsing L mem) prom prom.
-Proof.
-  exploit Memory.max_full_timemap_exists; eauto. intros [tm MAX].
-  dup CLOSED. inv CLOSED0. econs.
-  - i. dup GET. eapply MLE in GET0. eapply CLOSED1 in GET0. des.
-    exists to, from, msg.
-    destruct (classic (L loc)).
-    + dup GET. eapply MLE in GET0.
-      eapply not_latest_reserve_le_max_full_ts in GET0; eauto.
-      eapply or_strengthen in GET0. des; clarify.
-      * esplits; eauto.
-        { ii. unfold collapsed in *. des.
-          eapply caps_collapsing_ident3 in MAP0; eauto; cycle 1.
-          { eapply TimeFacts.lt_le_lt; eauto. } clarify.
-          assert (TO: to = ft).
-          { destruct TLE.
-            - eapply caps_collapsing_ident3 in MAP1; eauto.
-            - unfold Time.eq in *. clarify. inv MAP1; clarify.
-              + exfalso. eapply Time.lt_strorder.
-                eapply TimeFacts.lt_le_lt.
-                * eapply TLE0.
-                * eapply max_full_ts_le_max_ts; eauto.
-              + exfalso. eapply Time.lt_strorder.
-                eapply TimeFacts.lt_le_lt.
-                * etrans.
-                  { eapply Time.incr_spec. }
-                  { eapply TLE0. }
-                * eapply max_full_ts_le_max_ts; eauto. }
-          clarify. eapply Time.lt_strorder; eauto. }
-        { econs 2; eauto. }
-        { eapply caps_collapsing_message; eauto. }
-      * exfalso. exploit LATESTRESERVE; eauto.
-    + splits; auto.
-      * ii. unfold collapsed in *. des.
-        inv MAP0; clarify. inv MAP1; clarify.
-        eapply Time.lt_strorder. eauto.
-      * econs 1; eauto.
-      * eapply caps_collapsing_message; eauto.
-
-  - i. exists fto, ffrom, fmsg.
-    destruct (classic (L loc)).
-    + dup GET. eapply MLE in GET.
-      eapply not_latest_reserve_le_max_full_ts in GET; eauto.
-      des; clarify.
-      * splits; auto.
-        { eapply caps_collapsing_ident; eauto. }
-        { eapply caps_collapsing_ident; eauto.
-          etrans; eauto.
-          eapply memory_get_ts_strong in GET0. des; clarify.
-          { refl. }
-          { left. auto. } }
-      * exfalso. exploit LATESTRESERVE; eauto.
-    + splits; auto.
-      * econs 1; eauto.
-      * econs 1; eauto.
-Qed.
-
-Lemma other_collapsing_memory
-      mem0 mem1 mem2 prom (L: Loc.t -> Prop)
-      (MLE: Memory.le prom mem0)
-      (CLOSED: Memory.closed mem0)
-      (RESERVEWF: Memory.reserve_wf prom mem0)
-      (INHABITED: Memory.inhabited mem0)
-      (OTHERS: forall loc (SAT: L loc), Memory.latest_reserve loc prom mem0)
-      (CAP: Memory.cap prom mem0 mem1)
-      (FORGET: forget_memory (other_latest_reserves_times L mem0 \2/ other_caps_times L mem0 mem1) mem2 mem1)
-  :
-    memory_map (caps_collapsing L mem0) mem2 mem1.
-Proof.
-  exploit Memory.max_full_timemap_exists; eauto. intros [tm MAX].
-  dup CLOSED. inv CLOSED0. econs.
-  - i. destruct (classic (L loc)).
-    + dup GET. eapply forget_memory_get in GET0; eauto. des.
-Admitted.
 
 Inductive add_cap (caps: Loc.t -> option (Time.t * Time.t * Message.t)): Memory.t -> Memory.t -> Prop :=
 | add_cap_refl mem0
@@ -1185,6 +464,919 @@ Proof.
       exists mem_src, mem_src. splits; eauto.
       econs; eauto. econs; eauto.
 Qed.
+
+Definition collapsing_latest_reserves (L: Loc.t -> Prop)
+           (mem: Memory.t) (loc: Loc.t) (to: Time.t) (from: Time.t) :=
+  (<<LATEST: to = Memory.max_ts loc mem>>) /\
+  (<<RESERVE: Memory.get loc to mem = Some (from, Message.reserve)>>) /\
+  (<<OTHER: L loc>>)
+.
+
+Definition collapsing_latest_reserves_times (L: Loc.t -> Prop)
+           (mem: Memory.t) (loc: Loc.t) (to: Time.t): Prop :=
+  exists from,
+    (<<RESERVE: collapsing_latest_reserves L mem loc to from>>).
+
+Definition collapsing_caps (L: Loc.t -> Prop)
+           (mem0 mem1: Memory.t) (loc: Loc.t) (to: Time.t) (from: Time.t) :=
+  (<<FULL: Memory.max_full_ts mem0 loc from>>) /\
+  (<<LATEST: exists from0 val released,
+      (<<CAP: caps mem0 mem1 loc to from0 (Message.full val released)>>)>>) /\
+  (<<OTHER: L loc>>)
+.
+
+Definition collapsing_caps_times (L: Loc.t -> Prop)
+           (mem0 mem1: Memory.t) (loc: Loc.t) (to: Time.t) :=
+  exists from,
+    (<<CAP: collapsing_caps L mem0 mem1 loc to from>>).
+
+Definition times_in_memory (mem: Memory.t) (L: Loc.t -> list Time.t): Prop :=
+  forall loc t,
+    (<<SAT: List.In t (L loc)>>) <->
+    (<<INMEMORY:
+       (exists from msg, (<<GET: Memory.get loc t mem = Some (from, msg)>>)) \/
+       (exists to msg, (<<GET: Memory.get loc to mem = Some (t, msg)>>))>>).
+
+Lemma times_in_memory_exists mem
+  :
+    exists l, times_in_memory mem l.
+Proof.
+  hexploit (choice
+              (fun loc tl =>
+                 forall t,
+                   (<<SAT: List.In t tl>>) <->
+                   (<<INMEMORY:
+                      (exists from msg, (<<GET: Memory.get loc t mem = Some (from, msg)>>)) \/
+                      (exists to msg, (<<GET: Memory.get loc to mem = Some (t, msg)>>))>>))); auto.
+  intros loc.
+  hexploit (wf_cell_msgs_exists (mem loc)). i. des.
+  exists ((List.map (fun ftm =>
+                       match ftm with
+                       | (from, _, _) => from
+                       end) l)
+            ++
+            (List.map (fun ftm =>
+                         match ftm with
+                         | (_, to, _) => to
+                         end) l)).
+  i. split; i.
+  - red in H. eapply List.in_app_or in H. des.
+    + eapply List.in_map_iff in H. des.
+      destruct x as [[from to] msg]. clarify.
+      eapply COMPLETE in H0. right. eauto.
+    + eapply List.in_map_iff in H. des.
+      destruct x as [[from to] msg]. clarify.
+      eapply COMPLETE in H0. left. eauto.
+  - eapply List.in_or_app.  des.
+    + right. eapply COMPLETE in GET.
+      eapply List.in_map_iff. esplits; eauto. ss.
+    + left. eapply COMPLETE in GET.
+      eapply List.in_map_iff. esplits; eauto. ss.
+Qed.
+
+Inductive caps_collapsing (L: Loc.t -> Prop)
+          (mem: Memory.t): Loc.t -> Time.t -> Time.t -> Prop :=
+| caps_collapsing_not_in
+    loc t
+    (NSAT: ~ L loc)
+  :
+    caps_collapsing L mem loc t t
+| caps_collapsing_in_memory
+    loc t max
+    (SAT: L loc)
+    (FULL: Memory.max_full_ts mem loc max)
+    (TLE: Time.le t max)
+  :
+    caps_collapsing L mem loc t t
+| caps_collapsing_latest_reserve
+    loc t max
+    (SAT: L loc)
+    (FULL: Memory.max_full_ts mem loc max)
+    (MAX: t = Memory.max_ts loc mem)
+  :
+    caps_collapsing L mem loc max t
+| caps_collapsing_cap
+    loc t max
+    (SAT: L loc)
+    (FULL: Memory.max_full_ts mem loc max)
+    (CAP: t = Time.incr (Memory.max_ts loc mem))
+  :
+    caps_collapsing L mem loc max t
+| caps_collapsing_outer_memory
+    loc t
+    (SAT: L loc)
+    (TLE: Time.lt (Time.incr (Memory.max_ts loc mem)) t)
+  :
+    caps_collapsing L mem loc t t
+.
+
+Lemma forget_memory_get P mem0 mem1 loc to msg
+      (FORGET: forget_memory P mem0 mem1)
+      (GET: Memory.get loc to mem0 = Some msg)
+  :
+    (<<NOT: ~ P loc to>>) /\ (<<GET: Memory.get loc to mem1 = Some msg>>).
+Proof.
+  inv FORGET. destruct (classic (P loc to)).
+  - exfalso. rewrite FORGET0 in GET; auto. clarify.
+  - esplits; eauto.
+    rewrite <- COMPLETE; auto.
+Qed.
+
+Lemma caps_get_reserve mem0 prom mem1 loc to from
+      (RESERVE: Memory.reserve_wf prom mem0)
+      (INHABITED: Memory.inhabited mem0)
+      (CLOSED: Memory.closed mem0)
+      (CAP: Memory.cap prom mem0 mem1)
+      (CAPS: caps mem0 mem1 loc to from Message.reserve)
+  :
+    exists from0 to1 msg0 msg1,
+      (<<GET0: Memory.get loc from mem0 = Some (from0, msg0)>>) /\
+      (<<GET1: Memory.get loc to1 mem0 = Some (to, msg1)>>) /\
+      (<<SPACE: forall t (ITV: Interval.mem (from, to) t), ~ covered loc t mem0>>)
+.
+Proof.
+  unfold caps in CAPS. des. inv CAP.
+  exploit COMPLETE; eauto. i. des.
+  set (@cell_elements_least
+         (mem0 loc)
+         (fun t => Time.lt from t)). des.
+  - hexploit (MIDDLE loc f from from0 to0).
+    { econs; eauto. i.
+      destruct (Memory.get loc ts mem0) eqn:GET2; auto. destruct p.
+      exfalso. exploit LEAST.
+      - eapply GET2.
+      - eauto.
+      - i. exploit Memory.get_ts; try apply GET.
+        i. des; clarify.
+        + eapply Time.lt_strorder. eapply TimeFacts.lt_le_lt.
+          * eapply SAT.
+          * eapply Time.bot_spec.
+        + eapply Time.lt_strorder. eapply TimeFacts.le_lt_lt.
+          * etrans.
+            { eapply x1. }
+            { eapply TS2. }
+          * eauto. }
+    { exploit memory_get_from_mon.
+      - eapply x.
+      - eapply GET.
+      - eauto.
+      - i. destruct x2; auto. destruct H. exfalso.
+        exploit memory_get_from_inj.
+        { eapply SOUND. eapply GET. }
+        { eapply GET1. }
+        i. des; clarify.
+        + setoid_rewrite GET0 in GET. clarify.
+        + eapply Time.lt_strorder; eauto. }
+    i. exploit memory_get_from_inj.
+    { eapply H. }
+    { eapply GET1. }
+    i. des; clarify.
+    + esplits; eauto. ii. inv H0.
+      exploit Memory.get_disjoint.
+      * eapply SOUND. eapply GET2.
+      * eapply H.
+      * i. des; clarify. eapply x2; eauto.
+    + specialize (INHABITED loc).
+      eapply SOUND in INHABITED. clarify.
+  - exploit Memory.max_ts_spec.
+    { eapply x. }
+    i. des. destruct MAX.
+    + exfalso. eapply EMPTY; eauto.
+    + unfold Time.eq in *. subst. exploit x0; auto. intros LATEST.
+      exploit Memory.latest_val_exists; eauto. i. des.
+      exploit Memory.max_full_view_exists; eauto. i. des.
+      exploit BACK; eauto. i.
+      exploit memory_get_from_inj.
+      * eapply x1.
+      * eapply GET1.
+      * i. des; clarify.
+        { exfalso. eapply Time.lt_strorder. eapply TimeFacts.lt_le_lt.
+          - eapply Time.incr_spec.
+          - rewrite BOT0. eapply Time.bot_spec. }
+        { erewrite INHABITED in GET0. clarify. }
+Qed.
+
+Definition memory_concrete_le (lhs rhs: Memory.t): Prop :=
+  forall loc to from val released
+         (GET: Memory.get loc to lhs = Some (from, Message.full val released)),
+    Memory.get loc to rhs = Some (from, Message.full val released).
+
+Lemma memory_concrete_le_le
+  :
+    Memory.le <2= memory_concrete_le.
+Proof.
+  ii. eauto.
+Qed.
+Hint Resolve memory_concrete_le_le.
+
+Lemma memory_concrete_le_closed_timemap tm mem0 mem1
+      (MLE: memory_concrete_le mem0 mem1)
+      (TM: Memory.closed_timemap tm mem0)
+  :
+    Memory.closed_timemap tm mem1.
+Proof.
+  ii. hexploit (TM loc). i. des.
+  esplits; eauto.
+Qed.
+
+Lemma memory_concrete_le_closed_view vw mem0 mem1
+      (MLE: memory_concrete_le mem0 mem1)
+      (VW: Memory.closed_view vw mem0)
+  :
+    Memory.closed_view vw mem1.
+Proof.
+  inv VW. econs.
+  - eapply memory_concrete_le_closed_timemap; eauto.
+  - eapply memory_concrete_le_closed_timemap; eauto.
+Qed.
+
+Lemma memory_concrete_le_closed_opt_view vw mem0 mem1
+      (MLE: memory_concrete_le mem0 mem1)
+      (VW: Memory.closed_opt_view vw mem0)
+  :
+    Memory.closed_opt_view vw mem1.
+Proof.
+  inv VW; econs.
+  eapply memory_concrete_le_closed_view; eauto.
+Qed.
+
+Lemma memory_concrete_le_closed_msg msg mem0 mem1
+      (MLE: memory_concrete_le mem0 mem1)
+      (MSG: Memory.closed_message msg mem0)
+  :
+    Memory.closed_message msg mem1.
+Proof.
+  inv MSG; econs.
+  eapply memory_concrete_le_closed_opt_view; eauto.
+Qed.
+
+Lemma memory_concrete_le_closed_tview vw mem0 mem1
+      (MLE: memory_concrete_le mem0 mem1)
+      (VW: TView.closed vw mem0)
+  :
+    TView.closed vw mem1.
+Proof.
+  inv VW. econs.
+  - i. eapply memory_concrete_le_closed_view; eauto.
+  - eapply memory_concrete_le_closed_view; eauto.
+  - eapply memory_concrete_le_closed_view; eauto.
+Qed.
+
+Lemma memory_concrete_le_reserve_wf prom mem0 mem1
+      (MLE: memory_concrete_le mem0 mem1)
+      (RESERVE: Memory.reserve_wf prom mem0)
+  :
+    Memory.reserve_wf prom mem1.
+Proof.
+  ii. eapply RESERVE in GET. des.
+  esplits; eauto.
+Qed.
+
+Lemma memory_concrete_le_local_wf lc mem0 mem1
+      (MLE: memory_concrete_le mem0 mem1)
+      (PROM: Memory.le (Local.promises lc) mem1)
+      (LOCAL: Local.wf lc mem0)
+  :
+    Local.wf lc mem1.
+Proof.
+  inv LOCAL. econs; eauto.
+  - eapply memory_concrete_le_closed_tview; eauto.
+  - eapply memory_concrete_le_reserve_wf; eauto.
+Qed.
+
+Lemma partial_cap_closed prom mem0 mem1 mem2
+      (MLE: Memory.le prom mem0)
+      (CLOSED: Memory.closed mem0)
+      (RESERVEWF: Memory.reserve_wf prom mem0)
+      (INHABITED: Memory.inhabited mem0)
+      (CAP: Memory.cap prom mem0 mem2)
+      (MLE0: Memory.le mem0 mem1)
+      (MLE1: Memory.le mem1 mem2)
+  :
+    Memory.closed mem1.
+Proof.
+  exploit Memory.max_full_timemap_exists; eauto. intros [tm MAX].
+  inv CLOSED. econs; eauto.
+  i. destruct (Memory.get loc to mem0) as [[from0 msg0]|] eqn:GET.
+  - dup GET. eapply MLE0 in GET. clarify.
+    eapply CLOSED0 in GET0. des. esplits; eauto.
+    eapply memory_concrete_le_closed_msg; eauto.
+  - destruct msg.
+    + eapply MLE1 in MSG.
+      exploit caps_max_view; eauto.
+      * econs; eauto.
+      * i. des; clarify. esplits; eauto.
+        { econs; eauto. econs; eauto. econs. refl. }
+        { econs; eauto. ss. transitivity (Memory.max_ts loc mem0).
+          - specialize (MAX loc). inv MAX. des.
+            eapply Memory.max_ts_spec in GET0. des. eauto.
+          - left. eapply Time.incr_spec. }
+        { eapply memory_concrete_le_closed_msg; eauto.
+          econs. econs. econs.
+          - eapply Memory.max_full_timemap_closed; eauto.
+          - eapply Memory.max_full_timemap_closed; eauto. }
+    + esplits; eauto. econs.
+Qed.
+
+Lemma collapsing_caps_forget_le
+      mem0 mem1 mem2 prom (L: Loc.t -> Prop)
+      (CAP: Memory.cap prom mem0 mem2)
+      (FORGET: forget_memory (collapsing_latest_reserves_times L mem0 \2/ collapsing_caps_times L mem0 mem1) mem1 mem2)
+  :
+    memory_concrete_le mem0 mem1.
+Proof.
+  inv FORGET. ii.
+  erewrite COMPLETE.
+  - eapply Memory.cap_le in CAP; eauto. refl.
+  - ii. des.
+    + unfold collapsing_latest_reserves_times in *. des.
+      inv RESERVE. des. clarify.
+    + unfold collapsing_caps_times in *. des.
+      inv CAP0. des. unfold caps in CAP0. des. clarify.
+Qed.
+
+Definition collapsable_cap (L: Loc.t -> Prop) (prom mem: Memory.t): Prop :=
+  forall
+    loc (SAT: L loc)
+    from msg
+    (GET: Memory.get loc (Memory.max_ts loc mem) prom = Some (from, msg)),
+    msg <> Message.reserve.
+
+Lemma collapsing_caps_forget_prom_le
+      mem0 mem1 mem2 prom (L: Loc.t -> Prop)
+      (COLLAPSABLE: collapsable_cap L prom mem0)
+      (MLE: Memory.le prom mem0)
+      (CLOSED: Memory.closed mem0)
+      (RESERVEWF: Memory.reserve_wf prom mem0)
+      (INHABITED: Memory.inhabited mem0)
+      (CAP: Memory.cap prom mem0 mem2)
+      (FORGET: forget_memory (collapsing_latest_reserves_times L mem0 \2/ collapsing_caps_times L mem0 mem1) mem1 mem2)
+  :
+    Memory.le prom mem1.
+Proof.
+  inv FORGET. ii.
+  erewrite COMPLETE.
+  - eapply Memory.cap_le in CAP; eauto.
+  - ii. des.
+    + unfold collapsing_latest_reserves_times in *. des.
+      inv RESERVE. des. clarify.
+      dup LHS. eapply MLE in LHS0. clarify.
+      eapply COLLAPSABLE in OTHER. eapply OTHER in LHS. clarify.
+    + unfold collapsing_caps_times in *. des.
+      inv CAP0. des. unfold caps in CAP0. des.
+      eapply MLE in LHS; eauto. clarify.
+Qed.
+
+Lemma identity_mapped_view tm maxmap (f: Loc.t -> Time.t -> Time.t -> Prop)
+      (TM: TimeMap.le tm maxmap)
+      (IDENT: forall loc ts (TS: Time.le ts (maxmap loc)), f loc ts ts)
+  :
+    timemap_map f tm tm.
+Proof.
+  ii. eapply IDENT; eauto.
+Qed.
+
+Lemma caps_collapsing_ident L mem loc maxts ts
+      (MAX: Memory.max_full_ts mem loc maxts)
+      (TS: Time.le ts maxts)
+  :
+    (caps_collapsing L mem) loc ts ts.
+Proof.
+  i. destruct (classic (L loc)).
+  - econs 2; eauto.
+  - econs 1; eauto.
+Qed.
+
+Definition memory_reserve_wf mem := Memory.reserve_wf mem mem.
+
+Lemma memory_reserve_wf_promise
+      prom0 mem0 loc from to msg prom1 mem1 kind
+      (PROMISE: Memory.promise prom0 mem0 loc from to msg prom1 mem1 kind)
+      (RESERVE: memory_reserve_wf mem0)
+  :
+    memory_reserve_wf mem1.
+Proof.
+  inv PROMISE.
+  - ii. erewrite Memory.add_o in GET; eauto. des_ifs.
+    + ss; des; clarify. exploit RESERVE0; eauto.
+      i. des. eapply Memory.add_get1 in x; eauto.
+    + eapply RESERVE in GET; eauto. clear o. des.
+      eapply Memory.add_get1 in GET; eauto.
+  - ii. des. clarify. erewrite Memory.split_o in GET; eauto. des_ifs.
+    + ss; des; clarify. eapply Memory.split_get0 in MEM. des.
+      esplits; eauto.
+    + eapply RESERVE in GET; eauto. clear o o0. des.
+      eapply Memory.split_get1 in GET; eauto. des. esplits; eauto.
+  - ii. erewrite Memory.lower_o in GET; eauto. des_ifs.
+    + ss; des; clarify. inv MEM. inv LOWER. inv MSG_LE.
+    + eapply RESERVE in GET; eauto. clear o. des.
+      eapply Memory.lower_get1 in GET; eauto. des.
+      inv MSG_LE. esplits; eauto.
+  - ii. erewrite Memory.remove_o in GET; eauto. des_ifs. guardH o.
+    dup MEM. eapply Memory.remove_get0 in MEM0. des.
+    eapply RESERVE in GET; eauto. des. dup GET.
+    eapply Memory.remove_get1 in GET2; eauto. ss. des; clarify.
+    esplits; eauto.
+Qed.
+
+Lemma memory_reserve_wf_tstep lang (th0 th1: Thread.t lang) tf e
+      (RESERVE: memory_reserve_wf th0.(Thread.memory))
+      (STEP: Thread.step tf e th0 th1)
+  :
+    memory_reserve_wf th1.(Thread.memory).
+Proof.
+  inv STEP; inv STEP0; ss.
+  - inv LOCAL. eapply memory_reserve_wf_promise; eauto.
+  - inv LOCAL; eauto.
+    + inv LOCAL0. inv WRITE.
+      eapply memory_reserve_wf_promise; eauto.
+    + inv LOCAL1. inv LOCAL2. inv WRITE.
+      eapply memory_reserve_wf_promise; eauto.
+Qed.
+
+Lemma memory_reserve_wf_tsteps lang (th0 th1: Thread.t lang)
+      (RESERVE: memory_reserve_wf th0.(Thread.memory))
+      (STEP: rtc (tau (@Thread.step_allpf lang)) th0 th1)
+  :
+    memory_reserve_wf th1.(Thread.memory).
+Proof.
+  ginduction STEP; eauto.
+  i. eapply IHSTEP; eauto. inv H. inv TSTEP.
+  eapply memory_reserve_wf_tstep; eauto.
+Qed.
+
+Lemma memory_reserve_wf_init
+  :
+    memory_reserve_wf Memory.init.
+Proof.
+  ii. unfold Memory.get, Memory.init in *. ss.
+  rewrite Cell.init_get in GET. des_ifs.
+Qed.
+
+Lemma memory_reserve_wf_configuration_step c0 c1 e tid
+      (RESERVE: memory_reserve_wf c0.(Configuration.memory))
+      (STEP: Configuration.step e tid c0 c1)
+  :
+    memory_reserve_wf c1.(Configuration.memory).
+Proof.
+  eapply configuration_step_equivalent in STEP. inv STEP. ss.
+  eapply memory_reserve_wf_tstep in STEP0; eauto.
+  eapply memory_reserve_wf_tsteps in STEPS; eauto.
+Qed.
+
+Lemma not_latest_reserve_le_max_full_ts loc mem ts to from msg
+      (RESERVEWF : memory_reserve_wf mem)
+      (INHABITED : Memory.inhabited mem)
+      (MAX : Memory.max_full_ts mem loc ts)
+      (GET: Memory.get loc to mem = Some (from, msg))
+  :
+    (<<TLE: Time.le to ts>>) \/
+    ((<<TO: to = Memory.max_ts loc mem>>) /\
+     (<<FROM: from = ts>>) /\
+     (<<MSG: msg = Message.reserve>>)).
+Proof.
+  inv MAX. des.
+  destruct msg.
+  - left. eapply MAX0; eauto.
+  - exploit RESERVEWF; eauto. i. des.
+    destruct (TimeFacts.le_lt_dec to ts); auto.
+    dup x. eapply MAX0 in x; eauto. destruct x.
+    + exfalso. exploit memory_get_from_mon.
+      { eapply GET0. }
+      { eapply GET. }
+      { auto. }
+      i. eapply Time.lt_strorder. eapply TimeFacts.le_lt_lt.
+      * eapply x1.
+      * eapply H.
+    + unfold Time.eq in *. subst. right. esplits; eauto.
+      setoid_rewrite GET0 in x0. clarify.
+      dup GET. eapply Memory.max_ts_spec in GET1. des.
+      destruct MAX; auto. exfalso.
+      destruct msg.
+      * eapply MAX0 in GET2. eapply Time.lt_strorder.
+        eapply TimeFacts.lt_le_lt.
+        { etrans.
+          - eapply l.
+          - eapply H. }
+        { eauto. }
+      * dup GET2. eapply RESERVEWF in GET2. des.
+        eapply MAX0 in GET2.
+        exploit memory_get_from_mon.
+        { eapply GET. }
+        { eapply GET1. }
+        { eapply H. }
+        i. eapply Time.lt_strorder.
+        eapply TimeFacts.lt_le_lt.
+        { eapply l. }
+        { etrans.
+          - eapply x0.
+          - eapply Memory.get_ts in GET1. des; clarify. }
+Qed.
+
+Lemma max_full_ts_le_max_ts mem loc ts
+      (MAX: Memory.max_full_ts mem loc ts)
+  :
+    Time.le ts (Memory.max_ts loc mem).
+Proof.
+  inv MAX. des.
+  eapply Memory.max_ts_spec in GET. des; auto.
+Qed.
+
+Lemma max_full_ts_max_ts loc mem ts
+      (RESERVEWF : memory_reserve_wf mem)
+      (INHABITED : Memory.inhabited mem)
+      (MAX : Memory.max_full_ts mem loc ts)
+  :
+    (<<FULL: ts = Memory.max_ts loc mem>>) \/
+    ((<<TLT: Time.lt ts (Memory.max_ts loc mem)>>) /\
+     (<<GET: Memory.get loc (Memory.max_ts loc mem) mem = Some (ts, Message.reserve)>>)).
+Proof.
+  dup MAX. inv MAX. des.
+  eapply Memory.max_ts_spec in GET. des.
+  dup GET0. eapply not_latest_reserve_le_max_full_ts in GET0; eauto.
+  des; clarify.
+  - left. eapply TimeFacts.antisym; eauto.
+  - right. split; eauto. dup GET1.
+    eapply memory_get_ts_strong in GET1. des; clarify.
+    erewrite GET2 in *.
+    erewrite INHABITED in GET0. clarify.
+Qed.
+
+Lemma caps_collapsing_ident2 L mem maxts loc ts fts
+      (MAX: Memory.max_full_ts mem loc maxts)
+      (TS: Time.le fts maxts)
+      (MAP: (caps_collapsing L mem) loc ts fts)
+  :
+    ts = fts.
+Proof.
+  inv MAP; eauto.
+  - exploit Memory.max_full_ts_inj.
+    { eapply FULL. }
+    { eapply MAX. }
+    i. clarify. eapply TimeFacts.antisym; auto.
+    eapply max_full_ts_le_max_ts in FULL; auto.
+  - exfalso. eapply max_full_ts_le_max_ts in FULL. exfalso.
+    eapply Time.lt_strorder. eapply TimeFacts.lt_le_lt.
+    + eapply DenseOrder.DenseOrder.incr_spec.
+    + etrans.
+      * eapply TS.
+      * eapply max_full_ts_le_max_ts; eauto.
+Qed.
+
+Lemma caps_collapsing_ident3 L mem maxts loc ts fts
+      (RESERVEWF : memory_reserve_wf mem)
+      (INHABITED : Memory.inhabited mem)
+      (MAX: Memory.max_full_ts mem loc maxts)
+      (TS: Time.lt ts maxts)
+      (MAP: (caps_collapsing L mem) loc ts fts)
+  :
+    ts = fts.
+Proof.
+  inv MAP; eauto.
+  - exploit Memory.max_full_ts_inj.
+    { eapply FULL. }
+    { eapply MAX. }
+    i. clarify. exfalso. eapply Time.lt_strorder; eauto.
+  - exploit Memory.max_full_ts_inj.
+    { eapply FULL. }
+    { eapply MAX. }
+    i. clarify. exfalso. eapply Time.lt_strorder; eauto.
+Qed.
+
+Lemma caps_collapsing_timemap L mem tm
+      (INHABITED: Memory.inhabited mem)
+      (TM: Memory.closed_timemap tm mem)
+  :
+    timemap_map (caps_collapsing L mem) tm tm.
+Proof.
+  exploit Memory.max_full_timemap_exists; eauto. intros [maxmap MAX].
+  eapply identity_mapped_view.
+  - eapply Memory.max_full_timemap_spec; eauto.
+  - i. eapply caps_collapsing_ident; eauto.
+Qed.
+
+Lemma caps_collapsing_view L mem vw
+      (INHABITED: Memory.inhabited mem)
+      (VW: Memory.closed_view vw mem)
+  :
+    view_map (caps_collapsing L mem) vw vw.
+Proof.
+  inv VW. econs.
+  - eapply caps_collapsing_timemap; eauto.
+  - eapply caps_collapsing_timemap; eauto.
+Qed.
+
+Lemma caps_collapsing_opt_view L mem vw
+      (INHABITED: Memory.inhabited mem)
+      (VW: Memory.closed_opt_view vw mem)
+  :
+    opt_view_map (caps_collapsing L mem) vw vw.
+Proof.
+  inv VW; econs.
+  eapply caps_collapsing_view; eauto.
+Qed.
+
+Lemma caps_collapsing_message L mem msg
+      (INHABITED: Memory.inhabited mem)
+      (MSG: Memory.closed_message msg mem)
+  :
+    msg_map (caps_collapsing L mem) msg msg.
+Proof.
+  inv MSG; econs.
+  eapply caps_collapsing_opt_view; eauto.
+Qed.
+
+Lemma caps_collapsing_tview L mem vw
+      (INHABITED: Memory.inhabited mem)
+      (VW: TView.closed vw mem)
+  :
+    tview_map (caps_collapsing L mem) vw vw.
+Proof.
+  inv VW. econs.
+  - i. eapply caps_collapsing_view; eauto.
+  - eapply caps_collapsing_view; eauto.
+  - eapply caps_collapsing_view; eauto.
+Qed.
+
+Lemma caps_collapsing_promises (L: Loc.t -> Prop) mem prom
+      (MLE: Memory.le prom mem)
+      (CLOSED: Memory.closed mem)
+      (RESERVEWF: memory_reserve_wf mem)
+      (INHABITED: Memory.inhabited mem)
+      (LATESTRESERVE: forall
+          loc (SAT: L loc)
+          from msg
+          (GET: Memory.get loc (Memory.max_ts loc mem) prom = Some (from, msg)),
+          msg <> Message.reserve)
+  :
+    promises_map (caps_collapsing L mem) prom prom.
+Proof.
+  exploit Memory.max_full_timemap_exists; eauto. intros [tm MAX].
+  dup CLOSED. inv CLOSED0. econs.
+  - i. dup GET. eapply MLE in GET0. eapply CLOSED1 in GET0. des.
+    exists to, from, msg.
+    destruct (classic (L loc)).
+    + dup GET. eapply MLE in GET0.
+      eapply not_latest_reserve_le_max_full_ts in GET0; eauto.
+      eapply or_strengthen in GET0. des; clarify.
+      * esplits; eauto.
+        { ii. unfold collapsed in *. des.
+          eapply caps_collapsing_ident3 in MAP0; eauto; cycle 1.
+          { eapply TimeFacts.lt_le_lt; eauto. } clarify.
+          assert (TO: to = ft).
+          { destruct TLE.
+            - eapply caps_collapsing_ident3 in MAP1; eauto.
+            - unfold Time.eq in *. clarify. inv MAP1; clarify.
+              + exfalso. eapply Time.lt_strorder.
+                eapply TimeFacts.lt_le_lt.
+                * eapply TLE0.
+                * eapply max_full_ts_le_max_ts; eauto.
+              + exfalso. eapply Time.lt_strorder.
+                eapply TimeFacts.lt_le_lt.
+                * etrans.
+                  { eapply Time.incr_spec. }
+                  { eapply TLE0. }
+                * eapply max_full_ts_le_max_ts; eauto. }
+          clarify. eapply Time.lt_strorder; eauto. }
+        { econs 2; eauto. }
+        { eapply caps_collapsing_message; eauto. }
+      * exfalso. exploit LATESTRESERVE; eauto.
+    + splits; auto.
+      * ii. unfold collapsed in *. des.
+        inv MAP0; clarify. inv MAP1; clarify.
+        eapply Time.lt_strorder. eauto.
+      * econs 1; eauto.
+      * eapply caps_collapsing_message; eauto.
+  - i. exists fto, ffrom, fmsg.
+    destruct (classic (L loc)).
+    + dup GET. eapply MLE in GET.
+      eapply not_latest_reserve_le_max_full_ts in GET; eauto.
+      des; clarify.
+      * splits; auto.
+        { eapply caps_collapsing_ident; eauto. }
+        { eapply caps_collapsing_ident; eauto.
+          etrans; eauto.
+          eapply memory_get_ts_strong in GET0. des; clarify.
+          { refl. }
+          { left. auto. } }
+      * exfalso. exploit LATESTRESERVE; eauto.
+    + splits; auto.
+      * econs 1; eauto.
+      * econs 1; eauto.
+Qed.
+
+Lemma memory_cap_message_closed prom mem0 mem1
+      (CLOSED: Memory.closed mem0)
+      (CAP: Memory.cap prom mem0 mem1)
+      loc to from msg
+      (GET: Memory.get loc to mem1 = Some (from, msg))
+  :
+    Memory.closed_message msg mem0.
+Proof.
+  eapply Memory.cap_inv in GET; eauto. des.
+  - eapply CLOSED in GET. des; auto.
+  - clarify.
+  - clarify. econs. econs.
+    eapply Memory.max_full_view_closed; eauto.
+Qed.
+
+Lemma memory_get_ts_le loc to mem from msg
+      (GET: Memory.get loc to mem = Some (from, msg))
+  :
+    Time.le from to.
+Proof.
+  eapply Memory.get_ts in GET. des; clarify.
+  - refl.
+  - left. auto.
+Qed.
+
+Lemma caps_collapsing_memory
+      mem0 mem1 mem2 mem3 prom (L0 L1: Loc.t -> Prop)
+      (MLE: Memory.le prom mem0)
+      (CLOSED: Memory.closed mem0)
+      (RESERVEWF: Memory.reserve_wf prom mem0)
+      (RESERVEWF0: memory_reserve_wf mem0)
+      (INHABITED: Memory.inhabited mem0)
+      (COLLAPSABLE0: collapsable_cap L0 prom mem0)
+      (COLLAPSABLE1: collapsable_cap L1 prom mem0)
+      (DISJOINTLOC: forall l (SAT0: L0 l) (SAT1: L1 l) , False)
+      (CAP: Memory.cap prom mem0 mem1)
+      (FORGET0: forget_memory (collapsing_latest_reserves_times L0 mem0 \2/ collapsing_caps_times L0 mem0 mem1) mem2 mem1)
+      (FORGET1: forget_memory (collapsing_latest_reserves_times L1 mem0 \2/ collapsing_caps_times L1 mem0 mem1) mem3 mem2)
+  :
+    memory_map (caps_collapsing L1 mem0) mem3 mem2.
+Proof.
+  exploit Memory.max_full_timemap_exists; eauto. intros [tm MAX].
+  dup FORGET0. inv FORGET0. dup FORGET1. inv FORGET1.
+  dup CLOSED. inv CLOSED0. econs.
+  - i. dup GET. eapply forget_memory_get in GET0; eauto. des.
+    exists to, from, msg, msg.
+    destruct (classic (L1 loc)).
+    + esplits; eauto.
+      * econs 2; eauto.
+        eapply forget_memory_get in GET1; eauto. des.
+        apply not_or_and in NOT. apply not_or_and in NOT0. des.
+        dup GET0. eapply Memory.cap_inv in GET0; eauto. des; clarify.
+        { dup GET0. eapply not_latest_reserve_le_max_full_ts in GET0; eauto.
+          des; clarify. exfalso. eapply NOT. econs; eauto. econs; eauto. }
+        { inv GET2. dup GET5. eapply memory_get_ts_le in GET2.
+          eapply not_latest_reserve_le_max_full_ts in GET5; eauto. des.
+          - etrans; eauto.
+          - clarify. refl. }
+        { exfalso. eapply NOT2. econs; eauto. econs; eauto.
+          esplits; eauto. econs; eauto. }
+      * eapply caps_collapsing_message; eauto.
+        eapply forget_memory_get in GET1; eauto. des.
+        eapply memory_cap_message_closed in GET0; eauto.
+      * refl.
+    + esplits; eauto.
+      * econs 1; eauto.
+      * eapply caps_collapsing_message; eauto.
+        eapply forget_memory_get in GET1; eauto. des.
+        eapply memory_cap_message_closed in GET0; eauto.
+      * refl.
+  - i. destruct (classic (L1 loc)).
+    + destruct (classic ((collapsing_latest_reserves_times L1 mem0 \2/ collapsing_caps_times L1 mem0 mem1) loc fto)).
+      * des.
+        { inv H0. inv H1. des. clarify.
+          dup GET. eapply forget_memory_get in GET0; eauto. des.
+          dup RESERVE. eapply Memory.cap_le in RESERVE; eauto; [|refl]. clarify.
+
+
+          memory_map
+
+            Memory.get
+
+
+          dup GET1. eapply forget_memory_get in GET1; eauto. des.
+
+
+        admit.
+      * apply not_or_and in H0. des.
+        exists fto, ffrom, fmsg.
+        assert (TS: Time.le  fto (tm loc)).
+        { dup GET. eapply forget_memory_get in GET0; eauto. des.
+          dup GET1. eapply Memory.cap_inv in GET1; eauto. des; clarify.
+          - dup GET1. eapply not_latest_reserve_le_max_full_ts in GET1; eauto.
+            des; clarify. exfalso. eapply H0. econs; eauto. econs; eauto.
+          - inv GET2. dup GET5. eapply not_latest_reserve_le_max_full_ts in GET5; eauto.
+            des; clarify.
+            + eapply memory_get_ts_le in GET2. etrans; eauto.
+            + refl.
+          - exfalso. eapply H1. econs; eauto. econs; eauto.
+            esplits; eauto. econs; eauto. }
+        splits.
+        { econs 2; eauto. }
+        { erewrite COMPLETE0; eauto. ii. des; clarify. }
+        { econs 2; eauto. etrans; eauto. eapply memory_get_ts_le; eauto. }
+    + exists fto, ffrom, fmsg. esplits.
+      * econs 1; eauto.
+      * erewrite COMPLETE0; eauto. ii. des.
+        { inv H0. inv H1. des. clarify. }
+        { inv H0. inv H1. des. clarify. }
+      * econs 1; eauto.
+
+
+
+
+
+        Lemma caps_collapsing_memory
+      mem0 mem1 mem2 mem3 prom (L0 L1: Loc.t -> Prop)
+      (MLE: Memory.le prom mem0)
+      (CLOSED: Memory.closed mem0)
+      (RESERVEWF: Memory.reserve_wf prom mem0)
+      (INHABITED: Memory.inhabited mem0)
+      (COLLAPSABLE0: collapsable_cap L0 prom mem0)
+      (COLLAPSABLE1: collapsable_cap L1 prom mem0)
+      (DISJOINTLOC: forall l (SAT0: L0 l) (SAT1: L1 l) , False)
+      (CAP: Memory.cap prom mem0 mem1)
+      (FORGET0: forget_memory (collapsing_latest_reserves_times L0 mem0 \2/ collapsing_caps_times L0 mem0 mem1) mem2 mem1)
+      (FORGET1: forget_memory (collapsing_latest_reserves_times L1 mem0 \2/ collapsing_caps_times L1 mem0 mem1) mem3 mem2)
+  :
+    memory_map (caps_collapsing L1 mem0) mem3 mem2.
+Proof.
+  exploit Memory.max_full_timemap_exists; eauto. intros [tm MAX].
+  dup FORGET0. inv FORGET0. dup FORGET1. inv FORGET1.
+  dup CLOSED. inv CLOSED0. econs.
+  - i.
+
+
+    destruct (classic (L1 loc)).
+    + dup GET. eapply forget_memory_get in GET0; eauto. des.
+      e
+
+
+
+      admit.
+    + dup GET. eapply forget_memory_get in GET0; eauto. des.
+      exists to, from, msg, msg. esplits; eauto.
+      * econs 1; eauto.
+      * eapply caps_collapsing_message; eauto.
+        eapply forget_memory_get in GET1; eauto. des.
+        eapply memory_cap_message_closed in GET0; eauto.
+      * refl.
+  -  i.
+
+        eapply memory_concrete_le_closed_msg.
+        { eapply collapsing_caps_forget_le; eauto.
+
+        eapply forget_memory_get in GET1; eauto.
+
+      esplits; eauto.
+      * econs 1; eauto.
+      *
+
+
+      des.
+      dup GET1. erewrite <- COMPLETE0 in GET1; eauto. esplits; eauto.
+
+      admit.
+    +
+
+      dup inv FO
+
+Admitted.
+
+
+Lemma caps_collapsing_memory
+      mem0 mem1 mem2 mem3 prom (L0 L1: Loc.t -> Prop)
+      (MLE: Memory.le prom mem0)
+      (CLOSED: Memory.closed mem0)
+      (RESERVEWF: Memory.reserve_wf prom mem0)
+      (INHABITED: Memory.inhabited mem0)
+      (COLLAPSABLE0: collapsable_cap L0 prom mem0)
+      (COLLAPSABLE1: collapsable_cap L1 prom mem0)
+      (DISJOINTLOC: forall l (SAT0: L0 l) (SAT1: L1 l) , False)
+      (CAP: Memory.cap prom mem0 mem1)
+      (FORGET0: forget_memory (collapsing_latest_reserves_times L0 mem0 \2/ collapsing_caps_times L0 mem0 mem1) mem2 mem1)
+      (FORGET1: forget_memory (collapsing_latest_reserves_times (L0 \1/ L1) mem0 \2/ collapsing_caps_times (L0 \1/ L1) mem0 mem1) mem3 mem1)
+  :
+    memory_map (caps_collapsing L1 mem0) mem3 mem2.
+Proof.
+  (* exploit Memory.max_full_timemap_exists; eauto. intros [tm MAX]. *)
+  (* dup CLOSED. inv CLOSED0. econs. *)
+  (* - i. destruct (classic (L loc)). *)
+  (*   + dup GET. eapply forget_memory_get in GET0; eauto. des. *)
+Admitted.
+
+Lemma other_collapsing_memory
+      mem0 mem1 mem2 prom (L: Loc.t -> Prop)
+      (MLE: Memory.le prom mem0)
+      (CLOSED: Memory.closed mem0)
+      (RESERVEWF: Memory.reserve_wf prom mem0)
+      (INHABITED: Memory.inhabited mem0)
+      (COLLAPSABLE: collapsable_cap L prom mem0)
+      (CAP: Memory.cap prom mem0 mem1)
+      (FORGET: forget_memory (collapsing_latest_reserves_times L mem0 \2/ collapsing_caps_times L mem0 mem1) mem2 mem1)
+  :
+    memory_map (caps_collapsing L mem0) mem2 mem1.
+Proof.
+  exploit Memory.max_full_timemap_exists; eauto. intros [tm MAX].
+  dup CLOSED. inv CLOSED0. econs.
+  - i. destruct (classic (L loc)).
+    + dup GET. eapply forget_memory_get in GET0; eauto. des.
+Admitted.
+
 
 Lemma other_collapsing_memory
       mem0 mem1 mem2 prom (L: Loc.t -> Prop)
